Flapjack/Test/CompilerParity.lean
@@ -40,6 +40,7 @@ import Flapjack.Test.LoopEvaluateParity
 import Flapjack.Test.LoopObservationalSemanticsParity
 import Flapjack.Test.PanItreeFfiParity
 import Flapjack.Test.PanItreeTracePrefixParity
+import Flapjack.Test.PanItreeTracePrefix0Parity
 import Flapjack.Test.LoopCutStateParity
 import Flapjack.Test.LoopCutResParity
 import Flapjack.Test.LoopShMemLoadParity
@@ -675,6 +676,7 @@ def main : IO Unit := do
     Flapjack.Test.LoopObservationalSemanticsParity.runChecks,
     Flapjack.Test.PanItreeFfiParity.runChecks,
     Flapjack.Test.PanItreeTracePrefixParity.runChecks,
+    Flapjack.Test.PanItreeTracePrefix0Parity.runChecks,
     Flapjack.Test.LoopCutStateParity.runChecks,
     Flapjack.Test.LoopCutResParity.runChecks,
     Flapjack.Test.LoopShMemLoadParity.runChecks,
